src/study/Nemonuri.Study.CSharpSyntaxRewriter2.Modifier2/Nemonuri.StratifiedNodes.Factories.NodeLists.fst
@@ -1,6 +1,7 @@
 module Nemonuri.StratifiedNodes.Factories.NodeLists
 
 module L = FStar.List.Tot
+module Lp = FStar.List.Pure
 module I = Nemonuri.StratifiedNodes.Internals
 module N = Nemonuri.StratifiedNodes.Nodes
 module C = Nemonuri.StratifiedNodes.Children
@@ -13,6 +14,17 @@ module Fn = Nemonuri.StratifiedNodes.Factories.Nodes
 
 // https://learn.microsoft.com/en-us/dotnet/api/microsoft.codeanalysis.syntaxlist-1?view=roslyn-dotnet-4.12.0
 // https://github.com/dotnet/roslyn/blob/main/src/Compilers/Core/Portable/Syntax/SyntaxList%601.cs
+
+let rec create_leaf_node_list 
+  (#t:eqtype) (values:list t)
+  : Tot (N.node_list t)
+    (decreases values)
+  =
+  match values with
+  | [] -> []
+  | hd::tl -> 
+    (Fn.create_leaf_node hd)::
+    (create_leaf_node_list tl)
 
 let insert_range #t 
   (node_list:N.node_list t) 
@@ -102,10 +114,120 @@ let replace_range #t
 
 let replace #t
   (node_list:N.node_list t) 
-  (node:N.node t{ L.contains node node_list }) //
+  (node:N.node t{ L.contains node node_list })
   (inserting_node:N.node t)
   : Tot (N.node_list t)
   =
   replace_range node_list node [inserting_node]
+
+private let append #t (l1:list t) (l2:list t) 
+  : Pure (list t) True
+    (ensures fun r -> (L.length r) = (L.length l1 + L.length l2))
+  =
+  L.append_length l1 l2;
+  L.append l1 l2
+
+//#push-options "--split_queries always"
+(*
+let swap #t
+  (node_list:N.node_list t)
+  (index1:N.node_list_index node_list)
+  (index2:N.node_list_index node_list)
+  : Pure (N.node_list t) True
+    (ensures fun r -> 
+      ((L.length node_list) = (L.length r)) /\ (
+      match (index1 = index2) with
+      | true -> r = node_list
+      | false -> true
+    ))
+  =
+  match (index1 = index2) with
+  | true -> node_list
+  | false -> 
+  let (index_1st, index_2nd) = (
+    match (index1 < index2) with
+    | true -> (index1, index2)
+    | false -> (index2, index1)
+  ) in (
+    assert ((L.length node_list) >= 2);
+    assert (index_1st < index_2nd);
+    assert (index_1st < ((L.length node_list) - 1));
+
+    let (v1, v2) = L.splitAt index_1st node_list in
+    L.lemma_splitAt_snd_length index_1st node_list;
+    Lp.splitAt_length index_1st node_list;
+    assert ((L.length v1) = index_1st);
+    assert (((L.length v1) + (L.length v2)) = L.length node_list);
+    assert (Cons? v2);
+    let v2_head::v2_tail = v2 in
+    Lp.lemma_splitAt_index_hd index_1st node_list;
+    assert ((L.index node_list index_1st) = v2_head);
+
+    assert ((index_2nd - index_1st) >= 1);
+    let next_index = (index_2nd - index_1st - 1) in
+    let (v3, v4) = L.splitAt next_index v2_tail in
+    L.lemma_splitAt_snd_length next_index v2_tail;
+    Lp.splitAt_length next_index v2_tail;
+    assert (Cons? v4);
+    let v4_head::v4_tail = v4 in
+    (*
+    let q1_1 = (L.index v2_tail next_index) in
+    assert (q1_1 = v4_head);
+    let q1_2 = (L.index v2 (index_2nd - index_1st)) in
+    assert (q1_2 = q1_1);
+    Lp.lemma_splitAt node_list v1 v2 index_1st;
+    assert ((L.append v1 v2) == node_list);
+    L.index_extensionality (L.append v1 v2) node_list;
+    Lp.lemma_splitAt_reindex_right index_1st node_list (index_2nd - index_1st);
+    let q1_3 = (L.index node_list index_2nd) in
+    assert (q1_3 = q1_2);
+    *)
+    //Lp.lemma_splitAt_index_hd next_index v2_tail;
+    //Lp.lemma_splitAt_reindex_right index_1st node_list (index_2nd - index_1st);
+    //...아니 왜 뻗어버리면서 증명이 안 되냐...? 너무 길어서...?
+    assume ((L.index node_list index_2nd) = v4_head);
+
+    let r1 = ([v2_head] `append` v4_tail) in
+    assert (L.length r1 = L.length v4);
+    let r2 = (v3 `append` r1) in
+    assert (L.length r2 = L.length v2_tail);
+    let r3 = ([v4_head] `append` r2) in
+    assert (L.length r3 = L.length v2);
+    let r4 = (v1 `append` r3) in
+    assert (L.length r4 = (L.length v2 + L.length v1));
+    assert ((L.length v2 + L.length v1) = L.length node_list);
+    r4
+  )
+*)
+//#pop-options 
+
+// ...assert 는 나중에 필요한 것만 선택하기...
+let swap #t
+  (node_list:N.node_list t)
+  (index1:N.node_list_index node_list)
+  (index2:N.node_list_index node_list)
+  : Tot (N.node_list t)
+  =
+  match (index1 = index2) with
+  | true -> node_list
+  | false -> 
+  let (index_1st, index_2nd) = (
+    match (index1 < index2) with
+    | true -> (index1, index2)
+    | false -> (index2, index1)
+  ) in (
+    let (v1, v2) = L.splitAt index_1st node_list in
+    L.lemma_splitAt_snd_length index_1st node_list;
+    assert (Cons? v2);
+    let v2_head::v2_tail = v2 in
+
+    let next_index = (index_2nd - index_1st - 1) in
+    let (v3, v4) = L.splitAt next_index v2_tail in
+    L.lemma_splitAt_snd_length next_index v2_tail;
+    assert (Cons? v4);
+    let v4_head::v4_tail = v4 in
+
+    (v1 `append` [v4_head] `append` v3 `append` [v2_head] `append` v4_tail)
+  )
 
 //---|
